P5: add CmpNE64, CmpNE32, CmpLE64S conditions
Adds ne64 constructor to Cond type. CmpNE lowers to not(eq).
CmpLE64S uses signed bias trick (same as existing CmpLT32S).
Updates VexSyntax, VexIRParser, VexLowerCore, VexConcrete, VexBridgeCore.

Instances/ISAs/VexLowerCore.lean
@@ -68,6 +68,7 @@ def lowerCond {Reg : Type} [DecidableEq Reg] [Fintype Reg]
   | .eq64 lhs rhs => .eq (lowerExpr sub temps lhs) (lowerExpr sub temps rhs)
   | .lt64 lhs rhs => .lt (lowerExpr sub temps lhs) (lowerExpr sub temps rhs)
   | .le64 lhs rhs => .le (lowerExpr sub temps lhs) (lowerExpr sub temps rhs)
+  | .ne64 lhs rhs => .not (.eq (lowerExpr sub temps lhs) (lowerExpr sub temps rhs))
   | .amd64CalculateCondition code ccOp ccDep1 ccDep2 _ccNdep =>
       if code = 0x4 then
         lowerAmd64CalculateConditionZero
